\documentclass{basic}
\usepackage{mathtools}
\newcommand*\xor{\oplus}
\setlength{\parindent}{0pt}
\begin{document}

\(d(x_4 x_3 x_2 x_1 x_0, x_4 x_3 x_2 x_1 x_0) = 0\)\\
\(d(x_4 x_3 x_2 x_1 x_0, x_4 x_3 x_2 x_1 \bar{x_0}) = 1\)\\
\(d(x_4 x_3 x_2 x_1 x_0, x_4 x_3 x_2 \bar{x_1} x_0) = 2\)\\
\(d(x_4 x_3 x_2 x_1 x_0, x_4 x_3 x_2 \bar{x_1} \bar{x_0}) = 3\)\\
\(d(x_4 x_3 x_2 x_1 x_0, x_4 x_3 \bar{x_2} x_1 x_0) = 4\)\\
\(d(x_4 x_3 x_2 x_1 x_0, x_4 x_3 \bar{x_2} x_1 \bar{x_0}) = 5\)\\
\(d(x_4 x_3 x_2 x_1 x_0, x_4 x_3 \bar{x_2} \bar{x_1} x_0) = 6\)\\
\(d(x_4 x_3 x_2 x_1 x_0, x_4 x_3 \bar{x_2} \bar{x_1} \bar{x_0}) = 7\)\\
\(d(x_4 x_3 x_2 x_1 x_0, x_4 \bar{x_3} x_2 x_1 x_0) = 8\)\\
\(d(x_4 x_3 x_2 x_1 x_0, x_4 \bar{x_3} x_2 x_1 \bar{x_0}) = 9\)\\
\(d(x_4 x_3 x_2 x_1 x_0, x_4 \bar{x_3} x_2 \bar{x_1} x_0) = 10\)\\
\(d(x_4 x_3 x_2 x_1 x_0, x_4 \bar{x_3} x_2 \bar{x_1} \bar{x_0}) = 11\)\\
\(d(x_4 x_3 x_2 x_1 x_0, x_4 \bar{x_3} \bar{x_2} x_1 x_0) = 12\)\\
\(d(x_4 x_3 x_2 x_1 x_0, x_4 \bar{x_3} \bar{x_2} x_1 \bar{x_0}) = 13\)\\
\(d(x_4 x_3 x_2 x_1 x_0, x_4 \bar{x_3} \bar{x_2} \bar{x_1} x_0) = 14\)\\
\(d(x_4 x_3 x_2 x_1 x_0, x_4 \bar{x_3} \bar{x_2} \bar{x_1} \bar{x_0}) = 15\)\\
\(d(x_4 x_3 x_2 x_1 x_0, \bar{x_4} x_3 x_2 x_1 x_0) = 16\)\\
\(d(x_4 x_3 x_2 x_1 x_0, \bar{x_4} x_3 x_2 x_1 \bar{x_0}) = 17\)\\
\(d(x_4 x_3 x_2 x_1 x_0, \bar{x_4} x_3 x_2 \bar{x_1} x_0) = 18\)\\
\(d(x_4 x_3 x_2 x_1 x_0, \bar{x_4} x_3 x_2 \bar{x_1} \bar{x_0}) = 19\)\\
\(d(x_4 x_3 x_2 x_1 x_0, \bar{x_4} x_3 \bar{x_2} x_1 x_0) = 20\)\\
\(d(x_4 x_3 x_2 x_1 x_0, \bar{x_4} x_3 \bar{x_2} x_1 \bar{x_0}) = 21\)\\
\(d(x_4 x_3 x_2 x_1 x_0, \bar{x_4} x_3 \bar{x_2} \bar{x_1} x_0) = 22\)\\
\(d(x_4 x_3 x_2 x_1 x_0, \bar{x_4} x_3 \bar{x_2} \bar{x_1} \bar{x_0}) = 23\)\\
\(d(x_4 x_3 x_2 x_1 x_0, \bar{x_4} \bar{x_3} x_2 x_1 x_0) = 24\)\\
\(d(x_4 x_3 x_2 x_1 x_0, \bar{x_4} \bar{x_3} x_2 x_1 \bar{x_0}) = 25\)\\
\(d(x_4 x_3 x_2 x_1 x_0, \bar{x_4} \bar{x_3} x_2 \bar{x_1} x_0) = 26\)\\
\(d(x_4 x_3 x_2 x_1 x_0, \bar{x_4} \bar{x_3} x_2 \bar{x_1} \bar{x_0}) = 27\)\\
\(d(x_4 x_3 x_2 x_1 x_0, \bar{x_4} \bar{x_3} \bar{x_2} x_1 x_0) = 28\)\\
\(d(x_4 x_3 x_2 x_1 x_0, \bar{x_4} \bar{x_3} \bar{x_2} x_1 \bar{x_0}) = 29\)\\
\(d(x_4 x_3 x_2 x_1 x_0, \bar{x_4} \bar{x_3} \bar{x_2} \bar{x_1} x_0) = 30\)\\
\(d(x_4 x_3 x_2 x_1 x_0, \bar{x_4} \bar{x_3} \bar{x_2} \bar{x_1} \bar{x_0}) = 31\)\\
\end{document}
